

13712 107 126760/c

$$f: \{p_i, x_i, s_i\} \longrightarrow \{0, 1\} \quad : \wedge' \forall i \in \mathcal{I} \quad 1 \leq i \leq N = 100$$

$$p \in \mathbb{R}^+$$

$$P = \begin{pmatrix} 1 & 0 \\ 0 & 1 \end{pmatrix} \quad \text{or} \quad \begin{pmatrix} 1 & 0 \\ 0 & -1 \end{pmatrix} \quad .$$

$$x_i = \begin{cases} 7 & \text{if } i \text{ is a prime number} \\ 0 & \text{if } i \text{ is not a prime number} \end{cases}$$

[illegible]

$$\textcircled{1} \quad f(p_i, x_i = 0, S_i) = 1 \quad \Rightarrow \quad \text{for } 1 \leq i \leq N \quad \Rightarrow \quad x_{i+1} = 1$$

$\int_{\mathbb{R}^n} f(x) dx$

$$\textcircled{2} \quad f(p_i, x_i=1, s_i) = 1 \Rightarrow \int_{\text{join}} \kappa d \Rightarrow x_{i+1} = 1$$

$$\textcircled{3} \quad f(p_i, x_i=1, s_i) = 0 \Rightarrow \text{stop!!!} \Rightarrow x_{i+1} = 0$$

$$\textcircled{4} \quad f(p_i, x_i=0, s_i) = 0 \Rightarrow \int_{x_i=0}^{\infty} x_i f(x_i) dx_i = 0 \Rightarrow x_i = 0.$$

5, λ' d C760K : λN d13

(1/11) 317-131000 ①

λ' d C760K d λ'3 ; d10 d λN3 d1 ②

λN d10 317 ③

: 317 16100 ①

" 317 ← SMA20 - d λ'N λd10 λ'N d 317 = 5
 317 ← ~~SMA20~~ - d λ'N λ'N 317 317 317

(μ₂₀)_i SMA10

i	p _i	(μ ₂₀) _i SMA20
1	p ₁ = 10	μ ₁ = 10
2	p ₂	μ ₂
3	p ₃	μ ₃
4	p ₄	μ ₄
⋮		

ε = 0.001

②

$$f(p_i, \omega_i = 0, \{\mu_i\}) = \begin{cases} 0 & : p_i < \mu_i + \varepsilon \quad \lambda' d10 \lambda' \rightarrow x_{i+1} = 0 \\ 1 & : p_i > \mu_i + \varepsilon \quad 317 \rightarrow x_{i+1} = 1 \end{cases}$$

$$f(p_i, \omega_i = 1, \{\mu_i\}) = \begin{cases} 0 & : p_i < \mu_i + \varepsilon \quad 317 \rightarrow x_{i+1} = 0 \\ 1 & : p_i > \mu_i + \varepsilon \quad \lambda' d10 \lambda' \rightarrow x_{i+1} = 1 \end{cases}$$

i	P_i	SMA_{20} μ_i	position \downarrow x_i	ה'ב'י'ל'ו \downarrow f_i	S_i ה'ב'י'ל'ו \downarrow μ_i
1			0	0	0
2			0	0	0
3			0	0	0
4			0	0	0
5			0	0	0
6			0	1	
7			1	1	
8			1	1	
9			1	1	
10			1	1	
11			1	0	
12			0	0	
13			0	0	
14			0	0	
15			0	0	

ה'נ'נ'
ה'נ'נ'
↓

Buy

$j \rightarrow 6$
 $B = P_6$

ה'נ'נ'
ה'נ'נ'

↓
 $S = P_{11}$

SELL

$$S_6 (P_6 - B) = P_6 - B$$

$$S_7 (P_7 - B) = P_7 - B$$

$$S_8 (P_8 - B) = P_8 - B$$

ה'נ'נ' ה'נ'נ' ה'נ'נ'
 $F=1$! $X=0$ ע"כ

$$S_{11} (P_{11} - B) = P_{11} - B = a$$

$$a = S - B$$

a

a

$F=0$! $X=1$ ע"כ

ה'נ'נ' ה'נ'נ' ה'נ'נ' ה'נ'נ'
ה'נ'נ' ה'נ'נ'

